Replace the mini-protocol framework by a program-based one

src/Ouroboros-Mini_Protocols.thy
@@ -11,206 +11,308 @@ theory "Ouroboros-Mini_Protocols"
     Main
 begin
 
-subsection \<open>Foundations\<close>
+subsection \<open>Parties\<close>
 
 text \<open>
-  Perhaps surprisingly, there is no function for changing the alternative (left or right) of a sum
-  type value. We provide one here.
+  We introduce values for denoting parties that are not labeled with the absolute terms “client” and
+  “server” but the relative terms “us” and “them”. This enables us to sometimes use the same code
+  for handling clients and servers, as it depends on the viewpoint who “us” and “them” are.
 \<close>
 
-primrec sum_swap :: "'a + 'b \<Rightarrow> 'b + 'a" where
-  "sum_swap (Inl x) = Inr x" |
-  "sum_swap (Inr y) = Inl y"
+datatype party = Us | Them
 
-subsection \<open>State machines\<close>
+primrec other_party :: "party \<Rightarrow> party" where
+  "other_party Us = Them" |
+  "other_party Them = Us"
+
+subsection \<open>Inclusion of a “Done” Case\<close>
 
 text \<open>
-  State machines have final states (“done” states), which are special in that no party has agency in
-  them and no transitions may originate from them. Because of these special properties, there are
-  many situations where we want to deal with non-final states only. To account for that at the type
-  level, we work with types of proper, non-final, states and use a wrapper type that just adds a
-  single final state whenever we want to include such a state. We could use the \<^type>\<open>option\<close>
-  type for this purpose, with \<^const>\<open>None\<close> denoting the final state and \<^term>\<open>Some s\<close> denoting
-  the proper state~\<^term>\<open>s\<close>. However, this could quickly lead to confusion with the use of
-  \<^type>\<open>option\<close> for maps, which we use in state machine descriptions. Therefore, we introduce a
-  dedicated type \<open>successor\<close> that is isomorphic to \<^type>\<open>option\<close>. We use this type not only for
-  representing final \<^emph>\<open>states\<close> but also for representing other “final things”. An example are “done”
-  messages, which we want to distinguish from proper messages at the type level.
+  The original specification of mini-protocols uses “done” states and “done” messages to deal with
+  finalization of protocol execution. However, “done” \<^emph>\<open>states\<close> in particular are somewhat irregular
+  in that no party has agency in them and no transitions may originate from them. To simplify
+  matters, we exclude “done” states and “done” messages by default. Whenever we need to cover them,
+  we use a wrapper type that just adds a single value that denotes “done”. We could use the
+  \<^type>\<open>option\<close> type for this purpose, with \<^const>\<open>None\<close> denoting “done”. However, this could
+  quickly lead to confusion with the use of \<^type>\<open>option\<close> for maps, which we utilize in several
+  places in this theory. Therefore, we introduce a dedicated type \<open>or_done\<close> that is isomorphic to
+  \<^type>\<open>option\<close>. We use this type not only for “done” states and “done” messages but also for
+  representing other “final things”.
 \<close>
 
-datatype 'a successor = Done | Continuing 'a
+datatype 'a or_done = is_done: Done | Cont \<open>'a\<close>
 
 text \<open>
-  We introduce a type \<open>situation\<close> for describing the situations that pairs of communicating parties
-  can be in. At this point, we do not yet assign different roles to the parties, like client and
-  server or party with and party without agency, and instead just talk about party~1 and party~2.
-
-  The \<open>situation\<close> type has the following parameters:
-
-    \<^item> \<^typ>\<open>'s\<^sub>1\<close>, for the states where party~1 has agency
-
-    \<^item> \<^typ>\<open>'d\<^sub>1\<close>, for the mutable data (“internal mutable state”) maintained by party~1
-
-    \<^item> \<^typ>\<open>'s\<^sub>2\<close>, for the states where party~2 has agency
-
-    \<^item> \<^typ>\<open>'d\<^sub>2\<close>, for the mutable data (“internal mutable state”) maintained by party~2
-
-  Note that we distinguish between states according to agency at the type level. Whenever we want to
-  refer to states without any constraints on agency, we use the sum type \<^typ>\<open>'s\<^sub>1 + 's\<^sub>2\<close>.
+  It is generally not according to our style to introduce discriminators, but we need to introduce
+  one here (we chose \<^const>\<open>is_done\<close>) to permit corecursive invocations under \<open>case\<close> in
+  implementations of concrete mini-protocols. We discourage the explicit use of this discriminator.
 \<close>
 
-record ('s\<^sub>1, 'd\<^sub>1, 's\<^sub>2, 'd\<^sub>2) situation =
-  state :: "'s\<^sub>1 + 's\<^sub>2"
-  data :: "'d\<^sub>1 \<times> 'd\<^sub>2"
+subsection \<open>Possibilities\<close>
 
 text \<open>
-  We define the dual of a situation as this situation with the roles of the two parties swapped.
+  Before defining the notion of state machine, we introduce the more fundamental notion of
+  possibilities. Possibilities fully specify permitted communication patterns, but in contrast to
+  state machines they do not make explicit the states the communication can be in. They are somewhat
+  reminiscent of Conway’s games as discussed in \<^emph>\<open>On Numbers and Games\<close>.
 \<close>
 
-definition dual :: "('s\<^sub>1, 'd\<^sub>1, 's\<^sub>2, 'd\<^sub>2) situation \<Rightarrow> ('s\<^sub>2, 'd\<^sub>2, 's\<^sub>1, 'd\<^sub>1) situation" where
-  [simp]: "dual situation = \<lparr>state = sum_swap (state situation), data = prod.swap (data situation)\<rparr>"
+codatatype 'm possibilities =
+  Possibilities (agent: \<open>party\<close>) (can_finish: \<open>bool\<close>) (next_possibilities: \<open>'m \<rightharpoonup> 'm possibilities\<close>)
 
 text \<open>
-  We split the description of a state machine’s transitions into two parts according to the parties
-  that initiate the transitions. We call the transitions that can be initiated by a certain party
-  the steps of this party. The full specification of the transitions of a state machine then
-  consists of the client steps and the server steps of this state machine.
-
-  In the following, we first deal with steps before getting to complete transition systems.
-  Throughout our discussion of steps, we call the party to which certain steps belong the active
-  party and the other party the passive party.
+  Possibilities always denote a situation where at least one message will still be transmitted. The
+  \<^const>\<open>can_finish\<close> field being \<^const>\<open>True\<close> signals that it is possible for a “done” message
+  to be transmitted next.
 \<close>
 
 text \<open>
-  The basis for specifying steps is a type \<open>unchecked_steps\<close>. This type contains values that
-  describe steps but has also certain invalid members, which we later exclude by a subtype
-  construction.
-
-  The \<open>unchecked_steps\<close> type has the following parameters:
-
-    \<^item> \<^typ>\<open>'s\<^sub>a\<close>, for the states where the active party has agency
-
-    \<^item> \<^typ>\<open>'d\<^sub>a\<close>, for the mutable data maintained by the active party
-
-    \<^item> \<^typ>\<open>'m\<^sub>a\<close>, for the proper messages that the active party can send
-
-    \<^item> \<^typ>\<open>'s\<^sub>p\<close>, for the states where the passive party has agency
-
-    \<^item> \<^typ>\<open>'d\<^sub>p\<close>, for the mutable data maintained by the passive party
-
-  A value of type \<open>unchecked_steps\<close> is a record that consists of two fields:
-
-    \<^item> The \<open>initiation\<close> field states whether the active party, based on the current state and its own
-      mutable data, chooses to finish the execution of the mini-protocol and, if not, what proper
-      message it sends to the passive party and to what value it updates its mutable data.
-
-    \<^item> The \<open>completion\<close> field states to what state the system transitions if the active party sends a
-      given proper message while the system is in a given state and how the passive party updates
-      its mutable data upon receipt of this message. Not every pair of a message and a current state
-      has necessarily a follow-up state and a data update assigned to it, because there may be
-      messages that will not be sent in certain states and the \<open>completion\<close> field should not be
-      required to deal with situations that cannot occur. However, it is possible that the
-      \<open>completion\<close> field does not specify what to do with a message that \<^emph>\<open>can\<close> be sent in the
-      respective state. It is exactly this case where a value of type \<open>unchecked_steps\<close> is invalid.
-      The function \<open>unchecked_steps_are_valid\<close> defined after \<open>unchecked_steps\<close> makes this notion of
-      validity precise.
+  By swapping the notions of “us” and “them” and thus changing the viewpoint, we obtain the dual of
+  given possibilities.
 \<close>
 
-record ('s\<^sub>a, 'd\<^sub>a, 'm\<^sub>a, 's\<^sub>p, 'd\<^sub>p) unchecked_steps =
-  initiation :: "'s\<^sub>a \<Rightarrow> 'd\<^sub>a \<Rightarrow> ('m\<^sub>a \<times> 'd\<^sub>a) successor"
-  completion :: "'m\<^sub>a \<Rightarrow> 's\<^sub>a \<rightharpoonup> ('s\<^sub>a + 's\<^sub>p) \<times> ('d\<^sub>p \<Rightarrow> 'd\<^sub>p)"
-
-definition unchecked_steps_are_valid :: "('s\<^sub>a, 'd\<^sub>a, 'm\<^sub>a, 's\<^sub>p, 'd\<^sub>p) unchecked_steps \<Rightarrow> bool" where
-  [simp]: "unchecked_steps_are_valid \<S> =
-    (\<forall>s\<^sub>a d\<^sub>a m\<^sub>a d\<^sub>a'. initiation \<S> s\<^sub>a d\<^sub>a = Continuing (m\<^sub>a, d\<^sub>a') \<longrightarrow> s\<^sub>a \<in> dom (completion \<S> m\<^sub>a))"
+primcorec dual_possibilities :: "'m possibilities \<Rightarrow> 'm possibilities" (\<open>_\<^sup>\<bottom>\<close> [1000] 1000) where
+  "agent P\<^sup>\<bottom> = other_party (agent P)" |
+  "can_finish P\<^sup>\<bottom> = can_finish P" |
+  "next_possibilities P\<^sup>\<bottom> = map_option dual_possibilities \<circ> next_possibilities P"
 
 text \<open>
-  The meaning of a description of steps is a function that tells for a given current state where the
-  active party has agency and given current mutable data of the active and the passive party whether
-  as the next step the execution of the mini-protocol will be finished and, if not, what the
-  follow-up situation of the system will be. The \<open>unchecked_step\<close> function defined below provides
-  the meanings of all valid members of \<^type>\<open>unchecked_steps\<close>. We provide no guarantees regarding
-  its results for invalid members of \<^type>\<open>unchecked_steps\<close>.
+  We introduce a relation that tells what possibilities allow what messages to be transmitted next,
+  where messages include the “done” message.
+\<close>
+
+primrec permit :: "'m possibilities \<Rightarrow> 'm or_done \<Rightarrow> bool" (infix \<open>\<turnstile>\<close> 50) where
+  "P \<turnstile> Done \<longleftrightarrow> can_finish P" |
+  "P \<turnstile> Cont m \<longleftrightarrow> m \<in> dom (next_possibilities P)"
+
+text \<open>
+  Based on this relation, we introduce a function that tells when message transmission will end the
+  execution of the protocol and, in situations where it will not, what the possibilities afterwards
+  are.
+\<close>
+
+definition follow_up :: "'m possibilities \<Rightarrow> 'm or_done \<Rightarrow> 'm possibilities or_done" where
+  [simp]: "follow_up P M = map_or_done (the \<circ> next_possibilities P) M" if "P \<turnstile> M"
+
+subsection \<open>State Machines\<close>
+
+text \<open>
+  We define state machines as incomplete deterministic automatons that additionally assign agents to
+  states.
+\<close>
+
+record ('s, 'm) state_machine =
+  initial_state :: 's
+  agent_in_state :: "'s \<Rightarrow> party"
+  can_finish_in_state :: "'s \<Rightarrow> bool"
+  next_state :: "'s \<Rightarrow> 'm \<rightharpoonup> 's"
+
+text \<open>
+  Note that, analogously to possibilities, a state always denotes a situation where at least one
+  message will still be transmitted. The \<^const>\<open>can_finish_in_state\<close> function yielding
+  \<^const>\<open>True\<close> signals that it is possible for a “done” message to be transmitted next.
+\<close>
+
+text \<open>
+  By swapping the notions of “us” and “them” and thus changing the viewpoint, we obtain the dual of
+  a given state machine.
 \<close>
 
 definition
-  unchecked_step :: "
-    ('s\<^sub>a, 'd\<^sub>a, 'm\<^sub>a, 's\<^sub>p, 'd\<^sub>p) unchecked_steps \<Rightarrow>
-    's\<^sub>a \<Rightarrow>
-    'd\<^sub>a \<times> 'd\<^sub>p \<Rightarrow>
-    ('s\<^sub>a, 'd\<^sub>a, 's\<^sub>p, 'd\<^sub>p) situation successor"
+  dual_state_machine :: "('s, 'm) state_machine \<Rightarrow> ('s, 'm) state_machine"
+  ("_\<^sup>\<bottom>" [1000] 1000)
 where
-  [simp]: "unchecked_step \<S> s\<^sub>a d =
-    map_successor
-      (\<lambda>(m\<^sub>a, d\<^sub>a'). let (s', D) = the (completion \<S> m\<^sub>a s\<^sub>a) in \<lparr>state = s', data = (d\<^sub>a', D (snd d))\<rparr>)
-      (initiation \<S> s\<^sub>a (fst d))"
+  [simp]: "S\<^sup>\<bottom> = S \<lparr>agent_in_state := other_party \<circ> agent_in_state S\<rparr>"
 
 text \<open>
-  Based on the above developments, we define the type of steps, which contrary to
-  \<^type>\<open>unchecked_steps\<close> comes with a validity guarantee.
+  We define as the meaning of a state machine the possibilities corresponding to it. This means that
+  the essence of our state machine semantics is forgetting about states.
 \<close>
 
-typedef ('s\<^sub>a, 'd\<^sub>a, 'm\<^sub>a, 's\<^sub>p, 'd\<^sub>p) steps =
-  "{\<S> :: ('s\<^sub>a, 'd\<^sub>a, 'm\<^sub>a, 's\<^sub>p, 'd\<^sub>p) unchecked_steps. unchecked_steps_are_valid \<S>}"
-proof -
-  have "unchecked_steps_are_valid \<lparr>initiation = \<lambda>_ _. Done, completion = undefined\<rparr>"
+primcorec state_machine_semantics :: "('s, 'm) state_machine \<Rightarrow> 'm possibilities" (\<open>\<lbrakk>_\<rbrakk>\<close>) where
+  "agent \<lbrakk>S\<rbrakk> = agent_in_state S (initial_state S)" |
+  "can_finish \<lbrakk>S\<rbrakk> = can_finish_in_state S (initial_state S)" |
+  "next_possibilities \<lbrakk>S\<rbrakk> = map_option (\<lambda>s. \<lbrakk>S \<lparr>initial_state := s\<rparr>\<rbrakk>) \<circ> next_state S (initial_state S)"
+
+text \<open>
+  The state machine semantics preserves dualization.
+\<close>
+
+lemma state_machine_semantics_preserves_dualization:
+  fixes S :: "('s, 'm) state_machine"
+  shows "\<lbrakk>S\<^sup>\<bottom>\<rbrakk> = \<lbrakk>S\<rbrakk>\<^sup>\<bottom>"
+proof (coinduction arbitrary: S)
+  case Eq_possibilities
+  have "agent \<lbrakk>S\<^sup>\<bottom>\<rbrakk> = agent \<lbrakk>S\<rbrakk>\<^sup>\<bottom>"
     by simp
-  then show ?thesis
+  moreover
+  have "can_finish \<lbrakk>S\<^sup>\<bottom>\<rbrakk> = can_finish \<lbrakk>S\<rbrakk>\<^sup>\<bottom>"
+    by simp
+  moreover
+  have "
+    rel_option (\<lambda>P\<^sub>1 P\<^sub>2. \<exists>S' :: ('s, 'm) state_machine. P\<^sub>1 = \<lbrakk>S'\<^sup>\<bottom>\<rbrakk> \<and> P\<^sub>2 = \<lbrakk>S'\<rbrakk>\<^sup>\<bottom>)
+      (next_possibilities \<lbrakk>S\<^sup>\<bottom>\<rbrakk> m)
+      (next_possibilities \<lbrakk>S\<rbrakk>\<^sup>\<bottom> m)"
+    for m
+  proof (cases "next_state S (initial_state S) m")
+    case None
+    then show ?thesis
+      by simp
+  next
+    case (Some s)
+    define S' where "S' = S \<lparr>initial_state := s\<rparr>"
+    with Some have "next_possibilities \<lbrakk>S\<^sup>\<bottom>\<rbrakk> m = Some \<lbrakk>S'\<^sup>\<bottom>\<rbrakk>" and "next_possibilities \<lbrakk>S\<rbrakk>\<^sup>\<bottom> m = Some \<lbrakk>S'\<rbrakk>\<^sup>\<bottom>"
+      by (cases S, simp_all)
+    then show ?thesis
+      by (auto simp only: option.simps)
+  qed
+  ultimately show ?case
     by blast
 qed
 
-setup_lifting type_definition_steps
+subsection \<open>Programs\<close>
 
 text \<open>
-  The \<open>step\<close> function defined below provides the semantics of steps. It is the type-safe analog of
-  \<^const>\<open>unchecked_step\<close>.
+  A program implements either the client or the server part of a protocol.
 \<close>
 
-lift_definition
-  step :: "
-    ('s\<^sub>a, 'd\<^sub>a, 'm\<^sub>a, 's\<^sub>p, 'd\<^sub>p) steps \<Rightarrow>
-    's\<^sub>a \<Rightarrow>
-    'd\<^sub>a \<times> 'd\<^sub>p \<Rightarrow>
-    ('s\<^sub>a, 'd\<^sub>a, 's\<^sub>p, 'd\<^sub>p) situation successor"
-  is unchecked_step .
+codatatype ('M, 'r) program =
+  Return \<open>'r\<close> (\<open>\<triangle> _\<close> [56] 55) |
+  Send \<open>'M\<close> \<open>('M, 'r) program\<close> (\<open>\<up> _;/ _\<close> [0, 55] 55) |
+  Receive \<open>'M \<rightharpoonup> ('M, 'r) program\<close>
+
+syntax
+  "_Receive" :: "pttrn \<Rightarrow> ('M, 'r) program \<Rightarrow> ('M, 'r) program"
+  (\<open>\<down> _;/ _\<close> [0, 55] 55)
+translations
+  "\<down> M; \<Pi>" \<rightleftharpoons> "CONST Receive (\<lambda>M. \<Pi>)"
+print_translation \<open>
+  [Syntax_Trans.preserve_binder_abs_tr' \<^const_syntax>\<open>Receive\<close> \<^syntax_const>\<open>_Receive\<close>]
+\<close>
 
 text \<open>
-  As mentioned above, the transitions of a state machine are specified as a combination of the
-  client steps and the server steps of this state machine. We capture that by the type definition
-  below. Note that the type variables used in this type definition use indices \<open>c\<close> and~\<open>s\<close>, which
-  stand for “client” and “server”, respectively.
+  Note that we use the type variable~\<^typ>\<open>'M\<close> instead of~\<^typ>\<open>'m\<close> in the definition of
+  \<^type>\<open>program\<close> and the syntax declaration for \<^const>\<open>Receive\<close>. We do so to indicate that we
+  intend the corresponding type parameter to be instantiated with message types that include “done”
+  messages, that is, types of the form \<^typ>\<open>'m or_done\<close>. It might have been better to enforce the
+  possibility of sending and receiving “done” messages by defining \<^type>\<open>program\<close> as follows:\<^theory_text>\<open>
+    codatatype ('m, 'r) program =
+      Return \<open>'r\<close> (\<open>\<triangle> _\<close> [56] 55) |
+      Send \<open>'m or_done\<close> \<open>('m, 'r) program\<close> (\<open>\<up> _;/ _\<close> [0, 55] 55) |
+      Receive \<open>'m or_done \<rightharpoonup> ('m, 'r) program\<close>
+  \<close>
+  However, the construction of concrete programs will typically use the \<^emph>\<open>corec\<close> package, which
+  apparently cannot cope with this definition at present. The relevant issues are being discussed in
+  the mailing list thread that starts at
+  \<^url>\<open>https://lists.cam.ac.uk/sympa/arc/cl-isabelle-users/2023-08/msg00000.html\<close>.
 \<close>
-
-record ('s\<^sub>c, 'd\<^sub>c, 'm\<^sub>c, 's\<^sub>s, 'd\<^sub>s, 'm\<^sub>s) transitions =
-  client_steps :: "('s\<^sub>c, 'd\<^sub>c, 'm\<^sub>c, 's\<^sub>s, 'd\<^sub>s) steps"
-  server_steps :: "('s\<^sub>s, 'd\<^sub>s, 'm\<^sub>s, 's\<^sub>c, 'd\<^sub>c) steps"
 
 text \<open>
-  The meaning of a description of transitions is a function that tells for a given situation whether
-  as the next step the execution of the mini-protocol will be finished and, if not, what the
-  follow-up situation of the system will be. The semantics of transitions is provided by the
-  \<open>transition\<close> function.
+  We introduce a relation that tells what programs conform to what communication schemes, where a
+  communication scheme is either specified by possibilities or is a special “done” scheme, which
+  does not permit any further communication.
 \<close>
 
-definition
-  transition :: "
-    ('s\<^sub>c, 'd\<^sub>c, 'm\<^sub>c, 's\<^sub>s, 'd\<^sub>s, 'm\<^sub>s) transitions \<Rightarrow>
-    ('s\<^sub>c, 'd\<^sub>c, 's\<^sub>s, 'd\<^sub>s) situation \<Rightarrow>
-    ('s\<^sub>c, 'd\<^sub>c, 's\<^sub>s, 'd\<^sub>s) situation successor"
+coinductive
+  conforms_to :: "('m or_done, 'r) program \<Rightarrow> 'm possibilities or_done \<Rightarrow> bool"
+  (infix \<open>\<Colon>\<close> 50)
 where
-  [simp]: "transition \<T> \<sigma> = (
-    case state \<sigma> of
-      Inl s\<^sub>c \<Rightarrow> step (client_steps \<T>) s\<^sub>c (data \<sigma>) |
-      Inr s\<^sub>s \<Rightarrow> map_successor dual (step (server_steps \<T>) s\<^sub>s (prod.swap (data \<sigma>)))
-  )"
+  "\<triangle> _ \<Colon> Done" |
+  "\<up> M; \<Pi> \<Colon> Cont P"
+    if "agent P = Us" and "P \<turnstile> M" and "\<Pi> \<Colon> follow_up P M" |
+  "\<down> M; \<Xi> M \<Colon> Cont P"
+    if "agent P = Them" and "dom \<Xi> = {M. P \<turnstile> M}" and "\<forall>M \<in> dom \<Xi>. the (\<Xi> M) \<Colon> follow_up P M"
+
+subsection \<open>Protocols\<close>
 
 text \<open>
-  Finally, we specify that a state machine consists of an initial situation and state machine
-  transitions.
+  The communication patterns that a protocol permits are characterized by the possibilities of the
+  client and the server, where the latter have to be the dual of the former.
 \<close>
 
-record ('s\<^sub>c, 'd\<^sub>c, 'm\<^sub>c, 's\<^sub>s, 'd\<^sub>s, 'm\<^sub>s) state_machine =
-  initial :: "('s\<^sub>c, 'd\<^sub>c, 's\<^sub>s, 'd\<^sub>s) situation"
-  transitions :: "('s\<^sub>c, 'd\<^sub>c, 'm\<^sub>c, 's\<^sub>s, 'd\<^sub>s, 'm\<^sub>s) transitions"
+locale protocol_possibilities =
+  fixes client_possibilities :: "'m possibilities"
+  fixes server_possibilities :: "'m possibilities"
+  defines [simp]:
+    "server_possibilities \<equiv> client_possibilities\<^sup>\<bottom>"
+
+text \<open>
+  The permitted communication patterns of a protocol can be specified using state machines, from
+  which corresponding possibilities can be derived via the state machine semantics.
+\<close>
+
+locale protocol_state_machines =
+  fixes client_state_machine :: "('s, 'm) state_machine"
+  fixes server_state_machine :: "('s, 'm) state_machine"
+  defines [simp]:
+    "server_state_machine \<equiv> client_state_machine\<^sup>\<bottom>"
+begin
+
+definition client_possibilities :: "'m possibilities" where
+  [simp]: "client_possibilities = \<lbrakk>client_state_machine\<rbrakk>"
+
+definition server_possibilities :: "'m possibilities" where
+  [simp]: "server_possibilities = \<lbrakk>server_state_machine\<rbrakk>"
+
+sublocale protocol_possibilities \<open>client_possibilities\<close> \<open>server_possibilities\<close>
+  unfolding
+    client_possibilities_def and server_possibilities_def
+  and
+    server_state_machine_def and state_machine_semantics_preserves_dualization .
+
+end
+
+text \<open>
+  A protocol implementation consists of a client and a server program that conform to the
+  possibilities of the protocol.
+\<close>
+
+locale protocol_programs = protocol_possibilities +
+  fixes client_program :: "('m or_done, 'a) program"
+  fixes server_program :: "('m or_done, 'b) program"
+  assumes client_conformance:
+    "client_program \<Colon> Cont client_possibilities"
+  assumes server_conformance:
+    "server_program \<Colon> Cont server_possibilities"
+
+subsection \<open>Utilities\<close>
+
+text \<open>
+  When defining concrete possibilities, state machines, and programs, one often has to construct
+  partial functions that perform top-level case distinctions on message arguments. Implementing
+  such a partial function in a straightforward manner has the following issues:
+
+    \<^item> For each case where the partial function has a result, the implementation has to wrap this
+      result with \<^const>\<open>Some\<close>.
+
+    \<^item> The implementation must contain a default case where it returns \<^const>\<open>None\<close>.
+
+  To avoid these issues, we introduce the \<open>partial_case\<close> construct, which basically works like
+  \<open>case\<close> but adds the \<^const>\<open>Some\<close> wrapping and the \<^const>\<open>None\<close> case on the fly.
+\<close>
+
+nonterminal partial_case_clauses and partial_case_clause
+syntax
+  "_partial_case" :: "'a \<Rightarrow> partial_case_clauses \<Rightarrow> 'b option"
+  (\<open>(partial'_case _ of/ _)\<close> 10)
+syntax
+  "_more_partial_case_clauses" :: "partial_case_clause \<Rightarrow> partial_case_clauses \<Rightarrow> partial_case_clauses"
+  (\<open>_/ | _\<close>)
+syntax
+  "_one_partial_case_clause" :: "partial_case_clause \<Rightarrow> partial_case_clauses"
+  (\<open>_\<close>)
+syntax
+  "_partial_case_clause" :: "'a \<Rightarrow> 'b \<Rightarrow> partial_case_clause"
+  (\<open>(2_ \<Rightarrow>/ _)\<close> 10)
+translations
+  "_partial_case x Cs" \<rightharpoonup> "_case_syntax x Cs"
+translations
+  "_more_partial_case_clauses C Cs" \<rightharpoonup> "_case2 C Cs"
+translations
+  "_one_partial_case_clause C" \<rightharpoonup> "_case2 C (_case1 _ CONST None)"
+translations
+  "_partial_case_clause x y" \<rightharpoonup> "_case1 x (CONST Some y)"
+
+subsection \<open>The End\<close>
 
 end
